src/verification/stream_add.lean
@@ -14,7 +14,7 @@ variables {σ σ₁ σ₂ ι α : Type}
 @[simps]
 def Stream.add (a : Stream σ₁ ι α) (b : Stream σ₂ ι α) : Stream (σ₁ × σ₂) ι α :=
 { valid := λ s, a.valid s.1 ∨ b.valid s.2,
-  ready := λ s, a.ready s.1 ∨ b.ready s.2,
+  ready := λ s, (a.to_order s.1 ≤ b.to_order s.2 ∧ a.ready s.1) ∨ (b.to_order s.2 ≤ a.to_order s.1 ∧ b.ready s.2),
   next := λ s h, (if H : a.to_order s.1 ≤ b.to_order s.2 then a.next s.1 (valid_of_le_or h H) else s.1, 
                   if H : b.to_order s.2 ≤ a.to_order s.1 then b.next s.2 (valid_of_le_or h.symm H) else s.2),
   index := λ s h, option.get (show (min (a.index' s.1) (b.index' s.2)).is_some, by simpa),
@@ -60,25 +60,25 @@ lemma Stream.add.eval₀_left (h : a.to_order x < b.to_order y) (hva H) :
   (a +ₛ b).eval₀ (x, y) H = a.eval₀ x hva :=
 begin
   simp [Stream.eval₀, h.le, h.not_le],
-  by_cases H : a.ready x,
-  { simp [H, Stream.min_index h.le hva, Stream.value'_val H], },
-  { simp [H, Stream.value'], },
+  split_ifs with H,
+  { simp [Stream.min_index h.le hva, Stream.value'_val H], },
+  { refl, },
 end
 
 lemma Stream.add_eval₀_right (h : b.to_order y < a.to_order x) (hvb H) :
   (a +ₛ b).eval₀ (x, y) H = b.eval₀ y hvb :=
 begin
   simp [Stream.eval₀, h.le, h.not_le],
-  by_cases H : b.ready y,
+  split_ifs with H,
   { simp [H, Stream.min_index h.le hvb, Stream.value'_val H, min_comm (a.index' _) _], },
-  { simp [H, Stream.value'], },
+  { refl, },
 end
 
 lemma Stream.add_eval₀_both (h : a.to_order x = b.to_order y) (hva hvb H) :
   (a +ₛ b).eval₀ (x, y) H = a.eval₀ x hva + b.eval₀ y hvb :=
 begin
   simp [Stream.eval₀, h],
-  have : a.index _ hva = b.index _ hvb, { simpa [Stream.to_order, Stream.index'_val hva, Stream.index'_val hvb] using congr_arg prod.fst h, },
+  have : a.index _ hva = b.index _ hvb, { simpa [Stream.index'_val hva, Stream.index'_val hvb] using congr_arg prod.fst h, },
   by_cases H₁ : a.ready x; by_cases H₂ : b.ready y; simp [H₁, H₂, Stream.value', Stream.min_index h.le hva, this],
 end
 
@@ -106,8 +106,8 @@ begin
     obtain ⟨k₁, k₂, hk₁, hk₂, n_le, he, hiter⟩ := ih (a.next _ hvx) y (ha hvx) hb (by simpa [nat.succ_eq_one_add, add_assoc] using hn),
     refine ⟨k₁ + 1, k₂, nat.succ_le_succ hk₁, hk₂, _, _, _⟩,
     { ac_change _ ≤ k₁ + k₂ + 1, exact nat.succ_le_succ n_le, },
-    { simp [H, hvx], dsimp, simp [h.le, h.not_le, he, Stream.add.eval₀_left h hvx],
-      exact add_right_comm _ _ _, },
+    { dsimp, simp [h.le, h.not_le, he, Stream.add.eval₀_left h hvx, H, hvx],
+      apply add_right_comm, },
     simp [Stream.next'_val hvx, Stream.next'_val H, h.le, h.not_le, hiter], },
   { -- Advancing `b`
     have hvy : b.valid y := valid_of_le_or (or.symm H) h.le,
@@ -115,7 +115,7 @@ begin
     rw [Stream.bound_valid_succ] at hb,
     obtain ⟨k₁, k₂, hk₁, hk₂, n_le, he, hiter⟩ := ih x (b.next _ hvy) ha (hb hvy) (nat.le_of_succ_le_succ hn),
     refine ⟨k₁, k₂ + 1, hk₁, nat.succ_le_succ hk₂, nat.succ_le_succ n_le, _, _⟩,
-    { simp [H, hvy], dsimp, simp [h.le, h.not_le, he, Stream.add_eval₀_right h hvy, add_assoc], },
+    { dsimp, simp [H, hvy, h.le, h.not_le, he, Stream.add_eval₀_right h hvy, add_assoc], },
     simp [Stream.next'_val hvy, Stream.next'_val H, h.le, h.not_le, hiter], },
   { -- Advancing both `a` and `b`
     have hvx : a.valid x := valid_of_le_or H h.le,
@@ -127,7 +127,7 @@ begin
     obtain ⟨k₁, k₂, hk₁, hk₂, n_le, he, hiter⟩ := ih (a.next _ hvx) (b.next _ hvy) ((ha hvx).mono B₁.le_succ) (hb hvy) (nat.le_of_succ_le_succ hn),
     refine ⟨min (B₁ + 1) (k₁ + 1), k₂ + 1, min_le_left _ _, nat.succ_le_succ hk₂, succ_le_min_succ_add_succ n_le hk₁, _, _⟩,
     { rw Stream.eval_min_bound ha',
-      simp [H, hvx, hvy], dsimp, simp [h.le, h.symm.le, he, Stream.add_eval₀_both h hvx hvy],
+      dsimp, simp [h.le, h.symm.le, he, Stream.add_eval₀_both h hvx hvy, H, hvx, hvy],
       abel, },
     rw Stream.next'_min_bound ha',
     simp [h.le, h.symm.le, hiter, Stream.next'_val hvx, Stream.next'_val hvy, Stream.next'_val H], }
@@ -140,7 +140,7 @@ lemma Stream.add_spec' (a : Stream σ₁ ι α) (b : Stream σ₂ ι α) (x : σ
     ((a +ₛ b).next'^[B₁ + B₂] (x, y)) = (a.next'^[B₁] x, b.next'^[B₂] y) :=
 begin
   obtain ⟨k₁, k₂, hk₁, hk₂, H, he⟩ := Stream.add_spec a b _ _ (B₁ + B₂) ha hb rfl.le,
-  obtain ⟨rfl, rfl⟩ : k₁ = B₁ ∧ k₂ = B₂, { clear he, split; zify at *; linarith, }, 
+  obtain ⟨rfl, rfl⟩ : k₁ = B₁ ∧ k₂ = B₂, { clear he, split; linarith, }, 
   exact he,
 end
 
@@ -152,29 +152,35 @@ lemma StreamExec.add_bound_valid (a : StreamExec σ₁ ι α) (b : StreamExec σ
 by simpa [StreamExec.bound_valid, StreamExec.add, bound_valid_iff_next'_iterate,
   (Stream.add_spec' a.stream b.stream _ _ ha hb).2, not_or_distrib] using (and.intro ha hb) 
 
-lemma Stream.add_index_monotonic {a : Stream σ₁ ι α} {b : Stream σ₂ ι α}
-  (ha : a.monotonic) (hb : b.monotonic) {x y} (h : (a +ₛ b).valid (x, y)) :
-  (a +ₛ b).index' (x, y) ≤ (a +ₛ b).index' ((a +ₛ b).next (x, y) h) :=
+lemma Stream.add_monotonic {a : Stream σ₁ ι α} {b : Stream σ₂ ι α}
+  (ha : a.monotonic) (hb : b.monotonic) :
+  (a +ₛ b).monotonic :=
 begin
+  rintros ⟨x, y⟩ h,
   simp only [Stream.add_index'],
   refine min_le_min _ _,
-  { simp, split_ifs, { exact prod.lex.fst_le_of_le (ha _), }, exact rfl.le, },
-  { simp, split_ifs, { exact prod.lex.fst_le_of_le (hb _), }, exact rfl.le, },
+  { simp, split_ifs, { exact ha _, }, exact rfl.le, },
+  { simp, split_ifs, { exact hb _, }, exact rfl.le, },
 end
 
-lemma Stream.add_monotonic {a : Stream σ₁ ι α} {b : Stream σ₂ ι α}
-  (ha : a.monotonic) (hb : b.monotonic) : (a +ₛ b).monotonic :=
+lemma Stream.add_reduced {a : Stream σ₁ ι α} {b : Stream σ₂ ι α}
+  (ha : a.reduced) (hb : b.reduced) : (a +ₛ b).reduced :=
 begin
-  rintros ⟨x, y⟩ H,
-  
+  rintros ⟨x, y⟩ hv hr,
+  rcases hr with ⟨h, hr⟩|⟨h, hr⟩;
+  dsimp at hr h ⊢,
+  { simp [h, (show min (a.index' x) (b.index' y) = _, from min_eq_left (prod.lex.fst_le_of_le h))],
+    apply ne_min_of_ne_and_ne, { exact ha _ hr, },
+    split_ifs with H,
+    { obtain ⟨h₁, h₂⟩ : a.index' x = b.index' y ∧ (a.ready x ↔ b.ready y),
+      { simpa [Stream.to_order] using (antisymm h H), },
+      rw h₁, exact hb _ (by rwa ← h₂), },
+    exact ne_of_lt (prod.lex.fst_lt_of_lt_of_le (lt_of_le_not_le h H) (by simp [hr])), },
+  { simp [h, (show min (a.index' x) (b.index' y) = _, from min_eq_right (prod.lex.fst_le_of_le h))],
+    apply ne_min_of_ne_and_ne, swap, { exact hb _ hr, },
+    split_ifs with H,
+    { obtain ⟨h₁, h₂⟩ : a.index' x = b.index' y ∧ (a.ready x ↔ b.ready y),
+      { simpa [Stream.to_order] using (antisymm H h), },
+      rw ← h₁, exact ha _ (by rwa h₂), },
+    exact ne_of_lt (prod.lex.fst_lt_of_lt_of_le (lt_of_le_not_le h H) (by simp [hr])), },
 end
-
-/-
-lemma : ∀ n, ∃ (k₁ ≤ a.bound, k₂ ≤ b.bound), s.t. n ≤ k₁ + k₂ ∧ (a + b).eval_steps n = (a.eval_steps k₁ + b.eval_steps k₂)
-
-WLOG k₁, k₂ ≤ bound
-
-∀ n, ∃ (k₁ ≤ a.bound, k₂ ≤ b.bound), s.t. n ≤ k₁ + k₂ ∧ (a + b).eval_steps n = (a.eval_steps k₁ + b.eval_steps k₂)
-n = (a + b).bound = a.bound + b.bound
--/
-
